improve proof performance
- make valulen a parameter so it's really opaque.
- introduce an axiom that valulen=4096.
- use the axiom explicitly in addr2valu, valu2addr, and addr2valu2addr.

this prevents performance problems when expanding out valulen, but leaves
addrlen as-is, allowing better reasoning about addresses with [ring].

src/Prog.v
@@ -7,7 +7,8 @@ Set Implicit Arguments.
 (** * The programming language *)
 
 Definition addrlen := 64.
-Definition valulen := 4096.  (* 512 bytes *)
+Parameter valulen : nat.
+Axiom valulen_is: valulen = 4096.  (* 512 bytes *)
 
 Notation "'addr'" := (word addrlen).
 Notation "'valu'" := (word valulen).
